theories/concurrent/treiber_stack.v
@@ -106,7 +106,7 @@ Section treiber_stack_GS.
     wp_rec.
     iApply wp_fupd. wp_apply (wp_alloc with "[//]"). iIntros "%l (Hl & Hmeta)".
     iApply "HΦ".
-    iMod (auth_excl_alloc' []) as "(%γ & Hmodel₂ & Hmodel₁)".
+    iMod (auth_excl_alloc' (auth_excl_G := treiber_stack_G_model_G) []) as "(%γ & Hmodel₂ & Hmodel₁)".
     iMod (meta_set _ _ γ treiber_stack_meta_model with "Hmeta") as "#Hmeta"; first done.
     iSplitR "Hmodel₂"; iExists l, γ; iFrame "∗#"; last done.
     iSplitR; first done. iApply inv_alloc. iNext. iExists mlst_nil, []. iFrame "∗#".
@@ -140,7 +140,7 @@ Section treiber_stack_GS.
       iMod "HΦ" as "(%_vs1 & (%_l & %_γ & %Heq & #_Hmeta & Hmodel₂) & _ & HΦ)". injection Heq as <-.
       iDestruct (meta_agree with "Hmeta _Hmeta") as %<-. iClear "_Hmeta".
       iDestruct (auth_excl_agree_L with "Hmodel₂ Hmodel₁") as %->.
-      iMod (auth_excl_update' (v :: vs1) with "Hmodel₂ Hmodel₁") as "(Hmodel₂ & Hmodel₁)".
+      iMod (auth_excl_update' (auth_excl_G := treiber_stack_G_model_G) (v :: vs1) with "Hmodel₂ Hmodel₁") as "(Hmodel₂ & Hmodel₁)".
       iMod ("HΦ" with "[Hmodel₂] [//]") as "HΦ".
       { iExists l, γ. auto with iFrame. }
       iModIntro. iSplitL "Hl Hmodel₁".
@@ -218,7 +218,7 @@ Section treiber_stack_GS.
         iMod "HΦ" as "(%_vs1 & (%_l & %_γ & %Heq & #_Hmeta & Hmodel₂) & _ & HΦ)". injection Heq as <-.
         iDestruct (meta_agree with "Hmeta _Hmeta") as %<-. iClear "_Hmeta".
         iDestruct (auth_excl_agree_L with "Hmodel₂ Hmodel₁") as %->.
-        iMod (auth_excl_update' vs1 with "Hmodel₂ Hmodel₁") as "(Hmodel₂ & Hmodel₁)".
+        iMod (auth_excl_update' (auth_excl_G := treiber_stack_G_model_G) vs1 with "Hmodel₂ Hmodel₁") as "(Hmodel₂ & Hmodel₁)".
         iMod ("HΦ" with "[Hmodel₂] [//]") as "HΦ".
         { iRight. iExists v1, vs1. iSplit; first done. iExists l, γ. auto with iFrame. }
         iModIntro. iSplitL "Hl Hmodel₁".
